Tables/Table/Raw/JoinLemmas.lean
@@ -1,0 +1,29 @@
+module
+
+public import Tables.Table.Raw.Join
+import all Tables.Table.Raw.Join
+import Tables.Table.Raw.BasicLemmas
+
+public section
+
+namespace Tables.Table.Raw
+
+section wfColumnSize
+
+theorem wfColumnSize_distinct (self : Raw) (h : self.WfColumnSize) : (distinct self h).WfColumnSize := by
+  unfold distinct
+  apply wfColumnSize_ofRows
+
+theorem wfColumnSize_crossJoin (self other : Raw)
+    (h₁ : self.WfColumnSize) (h₂ : other.WfColumnSize) : (crossJoin self other h₁ h₂).WfColumnSize := by
+  unfold crossJoin
+  apply wfColumnSize_ofRows
+
+theorem wfColumnSize_leftJoin (self other : Raw) (keys : Array String)
+    (h₁ : self.WfColumnSize) (h₂ : other.WfColumnSize) : (leftJoin self other keys h₁ h₂).WfColumnSize := by
+  unfold leftJoin
+  apply wfColumnSize_ofRows
+
+end wfColumnSize
+
+end Tables.Table.Raw
